pcuic/theories/PCUICContextRelation.v
@@ -8,8 +8,8 @@ Ltac pcuic :=
   try repeat red; cbn in *;
    try (solve [ intuition auto; eauto with pcuic || (try lia || congruence) ]).
 
-Lemma context_relation_refl P : (forall Δ x, P Δ Δ x x) ->
-  forall Δ, context_relation P Δ Δ.
+Lemma All2_fold_refl P : (forall Δ x, P Δ Δ x x) ->
+  forall Δ, All2_fold P Δ Δ.
 Proof.
   intros HP.
   induction Δ.
@@ -17,34 +17,34 @@ Proof.
    destruct a as [? [?|] ?]; constructor; auto.
 Qed.
 
-Lemma context_relation_trans P :
+Lemma All2_fold_trans P :
   (forall Γ Γ' Γ'' x y z,
-      context_relation P Γ Γ' ->
-      context_relation P Γ' Γ'' ->
-      context_relation P Γ Γ'' ->
+      All2_fold P Γ Γ' ->
+      All2_fold P Γ' Γ'' ->
+      All2_fold P Γ Γ'' ->
       P Γ Γ' x y -> P Γ' Γ'' y z -> P Γ Γ'' x z) ->
-  Transitive (context_relation P).
+  Transitive (All2_fold P).
 Proof.
   intros HP x y z H. induction H in z |- *; auto;
   intros H'; unfold context in *; depelim H';
     try constructor; eauto; hnf in H0; noconf H0; eauto.
 Qed.
 
-Lemma context_relation_sym P :
+Lemma All2_fold_sym P :
   (forall Γ Γ' x y,
-      context_relation P Γ Γ' ->
-      context_relation P Γ' Γ ->
+      All2_fold P Γ Γ' ->
+      All2_fold P Γ' Γ ->
       P Γ Γ' x y -> P Γ' Γ y x) ->
-  Symmetric (context_relation P).
+  Symmetric (All2_fold P).
 Proof.
   intros HP x y H.
   induction H; constructor; auto.
 Qed.
 
-Lemma context_relation_app_inv {P} Γ Γ' Δ Δ' :
+Lemma All2_fold_app_inv {P} Γ Γ' Δ Δ' :
   #|Δ| = #|Δ'| ->
-  context_relation P (Γ ,,, Δ) (Γ' ,,, Δ') ->
-  context_relation P Γ Γ' * context_relation (fun Δ Δ' => P (Γ ,,, Δ) (Γ' ,,, Δ')) Δ Δ'.
+  All2_fold P (Γ ,,, Δ) (Γ' ,,, Δ') ->
+  All2_fold P Γ Γ' * All2_fold (fun Δ Δ' => P (Γ ,,, Δ) (Γ' ,,, Δ')) Δ Δ'.
 Proof.
   intros H.
   induction Δ in H, Δ', Γ, Γ' |- *;
@@ -56,135 +56,135 @@ Proof.
   constructor; auto.
 Qed.
 
-Lemma context_relation_app_inv_l {P} Γ Γ' Δ Δ' :
+Lemma All2_fold_app_inv_l {P} Γ Γ' Δ Δ' :
   #|Γ| = #|Γ'| ->
-  context_relation P (Γ ,,, Δ) (Γ' ,,, Δ') ->
-  context_relation P Γ Γ' * context_relation (fun Δ Δ' => P (Γ ,,, Δ) (Γ' ,,, Δ')) Δ Δ'.
+  All2_fold P (Γ ,,, Δ) (Γ' ,,, Δ') ->
+  All2_fold P Γ Γ' * All2_fold (fun Δ Δ' => P (Γ ,,, Δ) (Γ' ,,, Δ')) Δ Δ'.
 Proof.
   intros H.
   induction Δ in H, Δ', Γ, Γ' |- *;
   destruct Δ'; try discriminate.
   intuition auto. constructor.
-  intros H'; generalize (context_relation_length H'). simpl. len. lia.
-  intros H'; generalize (context_relation_length H'). simpl. len. lia.
+  intros H'; generalize (All2_fold_length H'). simpl. len. lia.
+  intros H'; generalize (All2_fold_length H'). simpl. len. lia.
   intros H'. simpl in H.
   specialize (IHΔ Γ Γ' Δ' ltac:(lia)).
   depelim H'; specialize (IHΔ H'); intuition auto;
   constructor; auto.
 Qed.
 
-Lemma context_relation_app {P} Γ Γ' Δ Δ' :
+Lemma All2_fold_app {P} Γ Γ' Δ Δ' :
   #|Δ| = #|Δ'| ->
-  context_relation P Γ Γ' -> context_relation (fun Δ Δ' => P (Γ ,,, Δ) (Γ' ,,, Δ')) Δ Δ' ->
-  context_relation P (Γ ,,, Δ) (Γ' ,,, Δ').
+  All2_fold P Γ Γ' -> All2_fold (fun Δ Δ' => P (Γ ,,, Δ) (Γ' ,,, Δ')) Δ Δ' ->
+  All2_fold P (Γ ,,, Δ) (Γ' ,,, Δ').
 Proof.
   intros H.
   induction 2; simpl; auto.
   constructor. apply IHX0. simpl in H. lia.
   apply p.
-  constructor. apply IHX0. simpl in H; lia.
-  apply p.
 Qed.
 
-Lemma context_relation_impl_onctx P P' Γ Δ Q :  
+Lemma All2_fold_impl_onctx P P' Γ Δ Q :  
   onctx Q Γ ->
-  context_relation P Γ Δ ->
+  All2_fold P Γ Δ ->
   (forall Γ Δ d d', 
-    context_relation P Γ Δ -> 
+    All2_fold P Γ Δ -> 
     P Γ Δ d d' ->
     ondecl Q d ->
     P' Γ Δ d d') ->
-  context_relation P' Γ Δ.
+  All2_fold P' Γ Δ.
 Proof.
   intros onc cr Hcr.
   induction cr; depelim onc; constructor; intuition eauto.
 Qed.
 
-Lemma context_relation_impl_ind P P' Γ Δ :  
-  context_relation P Γ Δ ->
+Lemma All2_fold_impl_ind P P' Γ Δ :  
+  All2_fold P Γ Δ ->
   (forall Γ Δ d d', 
-    context_relation P Γ Δ -> 
-    context_relation P' Γ Δ ->
+    All2_fold P Γ Δ -> 
+    All2_fold P' Γ Δ ->
     P Γ Δ d d' ->
     P' Γ Δ d d') ->
-  context_relation P' Γ Δ.
+  All2_fold P' Γ Δ.
 Proof.
   intros cr Hcr.
   induction cr; constructor; intuition eauto.
 Qed.
 
-Lemma context_relation_mapi P Γ Δ f g : 
-  context_relation (fun Γ Δ d d' =>
+Lemma All2_fold_mapi P Γ Δ f g : 
+  All2_fold (fun Γ Δ d d' =>
     P (mapi_context f Γ) (mapi_context g Δ) (map_decl (f #|Γ|) d) (map_decl (g #|Γ|) d')) Γ Δ 
-  <~> context_relation P (mapi_context f Γ) (mapi_context g Δ).
+  <~> All2_fold P (mapi_context f Γ) (mapi_context g Δ).
 Proof.
   split.
   - induction 1; simpl; constructor; intuition auto;
-    now rewrite <-(context_relation_length X).
-  - induction Γ as [|[na [b|] ty] Γ] in Δ |- *; destruct Δ as [|[na' [b'|] ty'] Δ]; simpl; intros H;
+    now rewrite <-(All2_fold_length X).
+  - induction Γ as [|d Γ] in Δ |- *; destruct Δ as [|d' Δ]; simpl; intros H;
     depelim H; constructor; simpl in *; auto.
-    * pose proof (context_relation_length H). len in H0.
-      now rewrite <- H0 in p.
-    * pose proof (context_relation_length H). len in H0.
-      now rewrite <- H0 in p.
+    pose proof (All2_fold_length H). len in H0.
+    now rewrite <- H0 in p.
 Qed.
 
-Lemma context_relation_map P Γ Δ f g : 
-  context_relation (fun Γ Δ d d' =>
+Lemma All2_fold_map P Γ Δ f g : 
+  All2_fold (fun Γ Δ d d' =>
     P (map_context f Γ) (map_context g Δ) (map_decl f d) (map_decl g d')) Γ Δ <~>
-  context_relation P (map_context f Γ) (map_context g Δ).
+  All2_fold P (map_context f Γ) (map_context g Δ).
 Proof.
   split.
   - induction 1; simpl; constructor; intuition auto;
-    now rewrite <-(context_relation_length X).
-  - induction Γ as [|[na [b|] ty] Γ] in Δ |- *; destruct Δ as [|[na' [b'|] ty'] Δ]; simpl; intros H;
+    now rewrite <-(All2_fold_length X).
+  - induction Γ as [|d Γ] in Δ |- *; destruct Δ as [|d' Δ]; simpl; intros H;
       depelim H; constructor; auto.
 Qed.
 
-Lemma context_relation_forallb2 (P : context_decl -> context_decl -> bool) Γ Δ : 
-  context_relation (fun _ _ => P) Γ Δ ->
+Lemma All2_fold_cst_map P Γ Δ f g : 
+  All2_fold (fun _ _ d d' => P (f d) (g d')) Γ Δ <~>
+  All2_fold (fun _ _ => P) (map f Γ) (map g Δ).
+Proof.
+  split.
+  - induction 1; simpl; constructor; intuition auto;
+    now rewrite <-(All2_fold_length X).
+  - induction Γ as [|d Γ] in Δ |- *; destruct Δ as [|d' Δ]; simpl; intros H;
+      depelim H; constructor; auto.
+Qed.
+
+Lemma All2_fold_forallb2 (P : context_decl -> context_decl -> bool) Γ Δ : 
+  All2_fold (fun _ _ => P) Γ Δ ->
   forallb2 P Γ Δ.
 Proof.
   induction 1; simpl; auto; now rewrite p, IHX.
 Qed.
 
-
-Lemma context_relation_nth {P n Γ Γ' d} :
-  context_relation P Γ Γ' -> nth_error Γ n = Some d ->
+Lemma All2_fold_nth {P n Γ Γ' d} :
+  All2_fold P Γ Γ' -> nth_error Γ n = Some d ->
   { d' & ((nth_error Γ' n = Some d') *
           let Γs := skipn (S n) Γ in
           let Γs' := skipn (S n) Γ' in
-          context_relation P Γs Γs' *
+          All2_fold P Γs Γs' *
           P Γs Γs' d d')%type }.
 Proof.
   induction n in Γ, Γ', d |- *; destruct Γ; intros Hrel H; noconf H.
   - depelim Hrel.
     simpl. eexists; intuition eauto.
-    eexists; intuition eauto.
   - depelim Hrel.
     destruct (IHn _ _ _ Hrel H).
     cbn -[skipn] in *.
     eexists; intuition eauto.
-    destruct (IHn _ _ _ Hrel H).
-    eexists; intuition eauto.
 Qed.
 
-Lemma context_relation_nth_r {P n Γ Γ' d'} :
-  context_relation P Γ Γ' -> nth_error Γ' n = Some d' ->
+Lemma All2_fold_nth_r {P n Γ Γ' d'} :
+  All2_fold P Γ Γ' -> nth_error Γ' n = Some d' ->
   { d & ((nth_error Γ n = Some d) *
         let Γs := skipn (S n) Γ in
         let Γs' := skipn (S n) Γ' in
-        context_relation P Γs Γs' *
+        All2_fold P Γs Γs' *
         P Γs Γs' d d')%type }.
 Proof.
   induction n in Γ, Γ', d' |- *; destruct Γ'; intros Hrel H; noconf H.
   - depelim Hrel.
     simpl. eexists; intuition eauto.
-    eexists; intuition eauto.
   - depelim Hrel.
     destruct (IHn _ _ _ Hrel H).
     cbn -[skipn] in *.
-    eexists; intuition eauto.
-    destruct (IHn _ _ _ Hrel H).
     eexists; intuition eauto.
 Qed.
